Wasm/Compiler.lean
@@ -20,11 +20,6 @@ def Expr.eval'' (e : Expr T) : { v : Val // v.toValType = T } := match e with
 | .I32Lit n => ⟨.I32 n, rfl⟩
 | .F32Lit n => ⟨.F32 n, rfl⟩
 | .I32Add lhs rhs => ⟨.I32 $ Val.toReprR lhs.eval'' + Val.toReprR rhs.eval'', rfl⟩
-      /- let ⟨lhs_e, hl⟩ := lhs.eval'' -/
-      /- let ⟨rhs_e, hr⟩ := rhs.eval'' -/
-      /- let hlr : lhs_e.toValType.repr = UInt32 := by rw [hl]; -/
-      /- let hrr : rhs_e.toValType.repr = UInt32 := by rw [hr]; -/
-      /- ⟨.I32 $ (val_repr ▸ lhs_e.toRepr) + (hrr ▸ rhs_e.toRepr), rfl⟩ -/
 | .I32Sub lhs rhs => ⟨.I32 $ Val.toReprR lhs.eval'' - Val.toReprR rhs.eval'', rfl⟩
 | .F32Add lhs rhs => ⟨.F32 $ Val.toReprR lhs.eval'' + Val.toReprR rhs.eval'', rfl⟩
 
@@ -92,99 +87,6 @@ theorem concat_nil_l {a b : StackTypes} {lhs : Prog a b} : Prog.concat lhs Prog.
 @[simp]
 theorem concat_nil_r {a b : StackTypes} {rhs : Prog a b} : Prog.concat Prog.nil rhs = rhs := rfl
 
-/- theorem concat_cons_eval {a b c: StackTypes} -/
-/-   (left : Prog a b) (right : Prog b c) {op : Op b s} {rrest : Prog s c} -/
-/-   (st : Stack) (h : st.types = a) -/
-/-   : (right = Prog.cons op rrest) -> -/
-/-       let ⟨lstack, lh⟩ := evalProg' left st h -/
-/-       let ⟨step, sh⟩ := evalOp' op lstack lh -/
-/-       let ⟨final, rh⟩ := evalProg' rrest step sh -/
-/-       evalProg' (Prog.concat left right) st h = evalProg' rrest step sh -/
-/- := by -/ 
-/-   simp; intro right_def; -/
-/-   induction left with -/
-/-   | nil => unfold evalProg'; simp; cases right with -/
-/-                                    | nil => contradiction; -/
-/-                                    | cons op' rrest' => rw [right_def, ← evalProg'.eq_def]; -/
-/-   | cons l_op lrest ih => unfold evalProg'; simp; cases right with -/
-/-                                                   | nil => contradiction; -/
-/-                                                   | cons op' rrest' => rw [right_def, <- evalProg'.eq_def]; sorry -/
-
-theorem concat_cons_eval {a b c: StackTypes}
-  (left : Prog a b) (op : Op b s) (rrest : Prog s c)
-  (st : Stack) (h : st.types = a)
-  :
-      let ⟨lstack, lh⟩ := evalProg' left st h
-      let ⟨step, sh⟩ := evalOp' op lstack lh
-      let ⟨final, rh⟩ := evalProg' rrest step sh
-      evalProg' (Prog.concat left (op ;; rrest)) st h = evalProg' rrest step sh
-:= by
-  simp; induction rrest with
-  | nil => conv => right; unfold evalProg';
-           conv => left; unfold evalProg' Prog.concat;
-           sorry
-  | cons op rest rest_ih => sorry
-
-theorem concat_eval {a b c : StackTypes} 
-  (left : Prog a b) (right : Prog b c) 
-  (astack : Stack) (ah : astack.types = a)
-  :
-    let ⟨bstack, bh⟩ := evalProg' left astack ah
-    evalProg' (Prog.concat left right) astack ah = evalProg' right bstack bh
-:= by
-  dsimp;
-  induction right with
-  | nil => aesop
-  | cons r_op rrest r_ih =>
-      rw [Subtype.ext_iff];
-      conv => right; unfold evalProg'; dsimp;
-      let ⟨lstack, lh⟩ := evalProg' left astack ah
-      let ⟨step, sh⟩ := evalOp' r_op lstack lh
-      let ⟨final, rh⟩ := evalProg' rrest step sh;
-      /- rw [concat_cons_eval]; -/
-
-  /- induction left with -/
-  /- | @nil s => -/
-  /-     conv => rhs; arg 2; rw [eval_nil]; -/
-  /-     unfold Prog.concat; -/ 
-  /-     rfl -/
-  /- | cons l_op lrest l_ih => -/
-  /-     have : -/ 
-      /- induction right with -/
-      /- | @nil s => rw [concat_nil]; rfl -/
-      /- | cons r_op rrest r_ih => -/
-      /-     conv => rhs; -/ 
-
-          
-
-        
-  /- obtain ⟨bstack, bh⟩ := (evalProg astack (ah ▸ left)) -/
-  /- show _ = _; -/
-  /- induction h : left generalizing astack with -/
-  /- | @nil s => -/ 
-
-  /-     sorry -/
-
--- TODO: rewrite without progResHead, insteal have smth like (eval e) :: stack
-/- theorem compile_head_eq_eval : ∀ (e : Expr T), eval_eq_compile e := by -/
-/-   intro e; unfold eval_eq_compile; intro prog compile_res; simp; -/
-/-   induction e with -/
-/-   | I32Lit n => -/
-/-       unfold progResHead; -/
-/-       have hc : compile_res = ⟨[Val.I32 n], by simp⟩ := by -/
-/-         (unfold compile_res; unfold prog Expr.compile evalProg evalOp evalProg; dsimp) -/
-/-       rw [hc]; dsimp; rfl; -/
-/-   | F32Lit n => -/
-/-       unfold progResHead; -/
-/-       have hc : compile_res = ⟨[Val.F32 n], by simp⟩ := by -/
-/-         (unfold compile_res; unfold prog Expr.compile evalProg evalOp evalProg; dsimp) -/
-/-       rw [hc]; dsimp; -/
-/-       unfold Expr.eval; rfl; -/
-/-   | I32Add lhs rhs lhs_ih rhs_ih => -/
-/-       have hc : compile_res = sorry := by ( -/
-/-         unfold compile_res prog Expr.compile; -/
-/-         unfold progResHead at *; -/
-
 theorem prog_eval_concat : evalProg' (Prog.concat l r) st h = evalProg' r (evalProg' l st h) h'
   := by
     induction l generalizing st with
@@ -198,30 +100,6 @@ theorem eval_prog_append : evalProg' (Prog.append l op) st h = evalOp' op (evalP
     induction l generalizing st with
     | nil => simp [evalProg']
     | cons l_op rest ih => simp [evalProg']; rw [ih];
-
-theorem compile_eq_eval {T : ValType} {stypes : StackTypes} {st : Stack} {h : st.types = stypes}
-  : ∀ (e : Expr T), (evalProg' e.compile st h).val = e.eval'.toVal :: st
-  := by
-      intro e;
-      induction e generalizing st stypes with
-      | I32Lit n => conv => left; simp [evalProg', Expr.compile, evalOp'];
-                    conv => right; simp [Expr.eval', TVal.toVal];
-      | F32Lit n => conv => left; simp [evalProg', Expr.compile, evalOp'];
-                    conv => right; simp [Expr.eval', TVal.toVal];
-      | I32Add lhs rhs ihl ihr =>
-          conv => left; unfold Expr.compile; rw [prog_append_assoc];
-          rw [prog_eval_concat];
-          · conv => left; arg 1; arg 2; rw [ihl];
-            rw [eval_prog_append];
-            rotate_left;
-            -- proving type hypotheses
-            · grind -- idk if this is a good use of grind
-            · grind
-            · conv => left; arg 1; arg 2; rw [ihr];
-              simp [Expr.eval'];
-              -- scuffed here bc of TVal/Val differences :/
-              unfold evalOp'; simp;
-              sorry
 
 theorem compile_eq_eval' {T : ValType} {stypes : StackTypes} {st : Stack} {h : st.types = stypes}
   : ∀ (e : Expr T), (evalProg' e.compile st h).val = e.eval''.val :: st
@@ -244,10 +122,28 @@ theorem compile_eq_eval' {T : ValType} {stypes : StackTypes} {st : Stack} {h : s
             · grind
             · conv => left; arg 1; arg 2; rw [ihr];
               conv => right; unfold Expr.eval'';
-              rw [eval_add] <;> grind
+              rw [eval_add] <;> grind;
       | I32Sub lhs rhs ihl ihr =>
-          sorry
-  /- have ⟨res, h⟩ := progResHead compile_res; -/
-  /- have h' : T.repr = res.toValType.repr := by rw [h]; -/
-  /- show (res.toRepr = h' ▸ e.eval); -/
-  /- induction e with -/
+          conv => left; unfold Expr.compile; rw [prog_append_assoc];
+          rw [prog_eval_concat];
+          · conv => left; arg 1; arg 2; rw [ihl];
+            rw [eval_prog_append];
+            rotate_left;
+            · grind
+            · grind;
+            · conv => left; arg 1; arg 2; rw [ihr];
+              conv => right; unfold Expr.eval'';
+              rw [eval_sub] <;> grind;
+      | F32Add lhs rhs ihl ihr =>
+          conv => left; unfold Expr.compile; rw [prog_append_assoc];
+          rw [prog_eval_concat];
+          · conv => left; arg 1; arg 2; rw [ihl];
+            rw [eval_prog_append];
+            rotate_left;
+            · grind
+            · grind
+            · conv => left; arg 1; arg 2; rw [ihr];
+              conv => right; unfold Expr.eval'';
+              rw [eval_add_f32] <;> grind;
+
+theorem compile_eq_eval : ∀ (e : Expr T), (evalProg' e.compile [] h).val = [e.eval''.val] := by simp [compile_eq_eval'];
